Finish definition of Kripke semantics

KripkeSemantics.v
@@ -1,16 +1,224 @@
-Require Import ssreflect stdpp.propset.
+Require Import ssreflect stdpp.boolset stdpp.propset stdpp.vector.
 
-Require Import Flowers.Syntax.
+Require Import Flowers.Utils Flowers.Terms Flowers.Syntax.
 
-Definition monotone {A B : Type} (f : A -> B) (RA : relation A) (RB : relation B) :=
+Record sig : Type := {
+  funs : boolset name;
+  preds : boolset name;
+  farity : ∀ f, f ∈ funs -> nat;
+  parity : ∀ p, p ∈ preds -> nat;
+}.
+
+Context (Σ : sig).
+
+(* Fixpoint twf (t : term) : bool :=
+  match t with
+  | TVar _ => true
+  | TFun f args =>
+      match decide (f ∈ Σ.(funs)) with
+      | left w => (length args =? Σ.(farity) f w) && forallb (twf <$> args)
+      | right _ => false
+      end
+  end. *)
+
+Inductive twf : term -> Type :=
+| twf_var n :
+    twf (TVar n)
+| twf_fun f args :
+    ∀ (Hf : f ∈ Σ.(funs)), ltwf args -> length args = Σ.(farity) f Hf ->
+    twf (TFun f args)
+with ltwf : list term -> Type :=
+| ltwf_nil :
+    ltwf []
+| ltwf_cons t l :
+    twf t -> ltwf l ->
+    ltwf (t :: l).
+
+Definition wfterm :=
+  { t : term & twf t }.
+
+(* Fixpoint wf (ϕ : flower) :=
+  match ϕ with
+  | Atom p args =>
+      match decide (p ∈ Σ.(preds)) with
+      | left w => (length args =? Σ.(parity) p w) && forallb (twf <$> args)
+      | right _ => false
+      end
+  | γ ⫐ Δ =>
+      let gwf '(n ⋅ Φ) := forallb (wf <$> Φ) in
+      gwf γ && forallb (gwf <$> Δ)
+  end. *)
+
+Inductive fwf : flower -> Type :=
+| fwf_atom p args :
+    ∀ (Hp : p ∈ Σ.(preds)), ltwf args -> length args = Σ.(parity) p Hp ->
+    fwf (Atom p args)
+| fwf_flower n Φ Δ :
+    wf Φ -> pwf Δ ->
+    fwf (n ⋅ Φ ⫐ Δ)
+with wf : bouquet -> Type :=
+| wf_nil : wf []
+| wf_cons ϕ Φ : fwf ϕ -> wf Φ -> wf (ϕ :: Φ)
+with pwf : list garden -> Type :=
+| pwf_nil : pwf []
+| pwf_cons n Φ Δ : wf Φ -> pwf Δ -> pwf ((n ⋅ Φ) :: Δ).
+
+Definition wfflower :=
+  { ϕ : flower & fwf ϕ }.
+
+Definition wfbouquet :=
+  { Φ : bouquet & wf Φ }.
+
+Definition elem {A C} `{Set_ A C} (X : C) :=
+  { x | x ∈ X }.
+
+Class premodel (D : Type) := {
+  domain : propset D;
+  interp_fun : ∀ (f : name) (H : f ∈ Σ.(funs)),
+    vec (elem domain) (Σ.(farity) f H) -> elem domain;
+  interp_pred : ∀ (p : name) (H : p ∈ Σ.(preds)),
+    propset (vec (elem domain) (Σ.(parity) p H));
+}.
+
+Lemma elem_subseteq {A : Type} (X Y : propset A) :
+  X ⊆ Y -> elem X -> elem Y.
+Proof.
+  move => H [x Hx]. exists x. exact (H x Hx).
+Defined.
+
+Lemma elem_subseteq_vec {A : Type} (X Y : propset A) :
+  X ⊆ Y -> ∀ n, vec (elem X) n -> vec (elem Y) n.
+Proof.
+  move => H. elim => [|n IH] xs.
+  * exact [#].
+  * inversion xs using (@vec_S_inv (elem X)).
+    move => {xs} [x Hx] xs.
+    constructor.
+    - exists x. exact (H x Hx).
+    - exact (IH xs).
+Defined.
+
+Definition premodel_incl {D} (M1 M2 : premodel D) : Prop.
+Proof.
+  refine { H : M1.(domain) ⊆ M2.(domain) | _ }.
+  refine (∀ (f : name) (w : f ∈ Σ.(funs)) (args : vec (elem M1.(domain)) (Σ.(farity) f w)), _ =@{elem M2.(domain)} _).
+  refine (elem_subseteq _ _ H (M1.(interp_fun) f w args)).
+  refine (M2.(interp_fun) f w (elem_subseteq_vec _ _ H _ args)).
+Defined.
+
+Section Eval.
+
+Context {D} (M : premodel D).
+
+Let dom := elem M.(domain).
+
+Definition eval := nat -> dom.
+
+Definition update (n : nat) (e1 e2 : eval) :=
+  fun m => if m <? n then e1 m else e2 (m - n).
+
+Fixpoint lapply_eval (e : eval) (l : list term) (H : ltwf l) {struct H} : vec dom (length l) :=
+  match H with
+  | ltwf_nil => vnil
+  | ltwf_cons x l Hx Hl =>
+      vcons (tapply_eval e x Hx) (lapply_eval e l Hl)
+  end
+with tapply_eval (e : eval) (t : term) (H : twf t) {struct H} : dom :=
+  match H with
+  | twf_var n => e n
+  | twf_fun f args Hf Hargs Hlen =>
+      interp_fun f Hf (vec_resize Hlen (lapply_eval e args Hargs))
+  end.
+
+End Eval.
+
+Definition monotone {A B : Type} (RA : relation A) (RB : relation B) (f : A -> B) :=
   ∀ x y, RA x y -> RB (f x) (f y).
 
-Class KStruct {A : Type} : Type := {
+Class KStruct (D : Type) : Type := {
   world : Type;
   accessible : relation world;
   accessible_po : PartialOrder accessible;
-  domain : world -> propset A;
-  domain_mono : monotone domain accessible subseteq;
-  interp : nat -> ∀ w, { a : A | a ∈ domain w };
-  forces : world -> flower;
+  model : world -> premodel D;
+  model_mono : monotone accessible premodel_incl model;
 }.
+
+Infix "≤" := accessible.
+
+Context {D} (K : KStruct D).
+
+Lemma eval_incl {α β} :
+  α ≤ β -> eval (model α) -> eval (model β).
+Proof.
+  move => H e.
+  refine (fun n => _).
+  case (model_mono α β H) => [Hincl _].
+  case (e n) => [a Ha].
+  exists a. by apply Hincl.
+Defined.
+
+(* Reserved Notation "α : e ⊩f ϕ" (at level 20, e at level 0).
+Reserved Notation "α : e ⊩ Φ" (at level 20, e at level 0).
+Reserved Notation "α : e ⊩p Δ" (at level 20, e at level 0).
+
+Inductive forces (α : world) (e : eval (model α)) : flower -> Prop :=
+
+| forces_atom p args Hp Hargs Hlen :
+    (vec_resize Hlen (lapply_eval (model α) e args Hargs)) ∈ interp_pred p Hp ->
+    α : e ⊩f Atom p args
+
+| forces_flower n Φ Δ :
+    (∀ β (H : α ≤ β), ∀ (en : eval (model β)),
+     let e' := update (model β) n en (eval_incl H e) in
+     β : e' ⊩ Φ -> β : e' ⊩p Δ) ->
+    α : e ⊩f (n ⋅ Φ ⫐ Δ)
+
+with bforces (α : world) (e : eval (model α)) : bouquet -> Prop :=
+
+with pforces (α : world) (e : eval (model α)) : list garden -> Prop :=
+
+where "α : e ⊩f ϕ" := (forces α e ϕ)
+  and "α : e ⊩ Φ" := (bforces α e Φ)
+  and "α : e ⊩p Δ" := (pforces α e Δ). *)
+
+Reserved Notation "α : e ⊩f ϕ ! H" (at level 20, e at level 0).
+Reserved Notation "α : e ⊩ Φ ! H" (at level 20, e at level 0).
+Reserved Notation "α : e ⊩p Δ ! H" (at level 20, e at level 0).
+
+Fixpoint fforces (α : world) (e : eval (model α)) (ϕ : flower) (H : fwf ϕ) : Prop :=
+  match H with
+  | fwf_atom p args Hp Hargs Hlen =>
+      (vec_resize Hlen (lapply_eval (model α) e args Hargs)) ∈ interp_pred p Hp
+  | fwf_flower n Φ Δ HΦ HΔ =>
+      ∀ β (H : α ≤ β), ∀ (en : eval (model β)),
+      let e' := update (model β) n en (eval_incl H e) in
+      β : e' ⊩ Φ ! HΦ -> β : e' ⊩p Δ ! HΔ
+  end
+
+with forces (α : world) (e : eval (model α)) (Φ : bouquet) (H : wf Φ) : Prop :=
+  match H with
+  | wf_nil =>
+      True
+  | wf_cons ϕ Φ Hϕ HΦ =>
+      α : e ⊩f ϕ ! Hϕ /\ α : e ⊩ Φ ! HΦ
+  end
+
+with pforces (α : world) (e : eval (model α)) (Δ : list garden) (H : pwf Δ) : Prop :=
+  match H with
+  | pwf_nil =>
+      False
+  | pwf_cons n Φ Δ HΦ HΔ =>
+      (∃ (en : eval (model α)), α : (update (model α) n en e) ⊩ Φ ! HΦ) \/
+      α : e ⊩p Δ ! HΔ
+  end
+
+where "α : e ⊩f ϕ ! H" := (fforces α e ϕ H)
+  and "α : e ⊩ Φ ! H" := (forces α e Φ H)
+  and "α : e ⊩p Δ ! H" := (pforces α e Δ H).
+
+Definition entails (Φ Ψ : wfbouquet) :=
+  let '(existT Φ HΦ) := Φ in
+  let '(existT Ψ HΨ) := Ψ in
+  ∀ α e, α : e ⊩ Φ ! HΦ -> α : e ⊩ Ψ ! HΨ.
+
+Infix "⊨" := entails (at level 40).
