Terms.v
@@ -9,45 +9,6 @@ Inductive term :=
 | TVar (n : nat)
 | TFun (f : name) (args : list term).
 
-(* Definition sig : Type :=
-  name -> option nat.
-
-Context (Σ : sig).
-
-Definition andb_map {A} (f : A -> bool) (l : list A) : bool :=
-  foldr (λ x b, b && f x) true l.
-
-Lemma andb_map_In {A} {f : A -> bool} {x : A} : ∀ (l : list A),
-  In x l -> andb_map f l -> f x.
-Proof.
-  elim => [Hx H |a l IH Hx H].
-  * elim Hx.
-  * elim Hx => [Heq |HIn];
-    rewrite /andb_map//= in H; apply andb_prop_elim in H.
-    - rewrite -Heq; easy.
-    - apply IH; easy.
-Qed.
-
-Fixpoint wf (t : fterm) : bool :=
-  match t with
-  | TVar _ => true
-  | TFun f args =>
-      Σ (f, length args) && andb_map wf args
-  end.
-
-Definition term :=
-  { t : fterm | wf t }. *)
-
-(* Lemma wf_fun_inv f : ∀ args,
-  wf (TFun f args) -> Forall wf args.
-Proof.
-  move => args Hwf.
-  apply In_Forall. move => t HIn.
-  apply (andb_map_In args); auto.
-  rewrite /wf in Hwf.
-  apply andb_prop_elim in Hwf. easy.
-Qed. *)
-
 Lemma term_induction_full :
   ∀ (P : term -> Prop) (Pn : nat -> Prop)
   (IHn : ∀ n, Pn n)
